@prefix rdf:        <http://www.w3.org/1999/02/22-rdf-syntax-ns#> .
@prefix rdfs:       <http://www.w3.org/2000/01/rdf-schema#> .
@prefix dc:         <http://purl.org/dc/elements/1.1/> .
@prefix dtype:      <http://www.w3.org/2001/XMLSchema#> . 
@prefix owl:        <http://www.w3.org/2002/07/owl#> .
@prefix :           <http://www.w3.org/2004/09/fresnel#>  .

# -----------------------------------------------
# About this document
<http://www.w3.org/2004/09/fresnel-extended> a owl:Ontology ;
    owl:imports      <http://www.w3.org/2004/09/fresnel> ;
    rdfs:comment     "Extended Lens and Style Vocabulary"@en ;
    dc:description   "Vocabulary for relating and grouping lenses and styles."@en ;
    dc:date          "2005-03-09"^^dtype:date ;
    dc:format        "RDF"@en ;
    dc:creator        "Chris Bizer <chris@bizer.de>"^^dtype:string ;
    dc:creator        "Ryan Lee <ryanlee@w3.org>"^^dtype:string ;
    dc:creator        "Stefano Mazzocchi <stefanom@mit.edu>"^^dtype:string ;
    dc:creator        "Emmanuel Pietriga <emmanuel.pietriga@inria.fr>"^^dtype:string ;
    dc:identifier     <http://www.w3.org/2004/09/fresnel-extended#> ;
    owl:versionInfo   "$Id: extended.owl.n3 5461 2006-11-17 19:39:18Z ryanlee $"^^dtype:string
    .
   
#@@@TODO:
# - add containerStyle 
# - resolve style/format discrepancies
# - add in any redefinition needed for *Style / *Format properties

# --------------------------------------------------------------   
# Extended Lens Vocabulary 
# --------------------------------------------------------------     
# Contents:
#     1. Lens Inheritance Vocabulary 
#     2. Property Description Vocabulary
#     3. Lens Relation Vocabulary

# -----------------------------------------------
# 1. Lens Inheritance Vocabulary 
# -----------------------------------------------

# @@@ things that could only take resources in core can now
#     take literals - redefine?  forget the import?
:Lens rdfs:subClassOf [
        a owl:Restriction ;
        owl:onProperty :extends;
        owl:minCardinality "0"^^dtype:nonNegativeInteger ;
    ] ;
    rdfs:subClassOf [
        a owl:Restriction ;
        owl:onProperty :extends;
        owl:maxCardinality "1"^^dtype:nonNegativeInteger
    ] ;
    # @@@ work on
    rdfs:subClassOf [
        a owl:Restriction ;
        owl:onProperty :use ;
        owl:minCardinality "0"^^dtype:nonNegativeInteger ;
    ] ;
    # @@@ work on
    rdfs:subClassOf [
        a owl:Restriction ;
        owl:onProperty :moreDetailsFor ;
        owl:minCardinality "0"^^dtype:nonNegativeInteger ;
    ] ;
    rdfs:subClassOf [
        a owl:Restriction ;
        owl:onProperty :moreDetailsFor ;
        owl:allValuesFrom :Lens
    ]
    .

#:extends a owl:ObjectProperty ;
#    rdfs:label "extends"@en ;
#    rdfs:comment "Extends allows you to model inheritance relation between lenses.  No multiple inheritance; browser detects and stops on loops."@en ;
#    rdfs:domain :Lens ;
#    rdfs:range :Lens
#    .

# @@@ can be used in a :PropertyList - redefine PropertyList?
#:super a owl:Thing ;
#    rdfs:label "Super"@en ;
#    rdfs:comment "Ordered List of all properties which are defined by the super lens."@en
#    .

# -----------------------------------------------
# 2. Property Description Vocabulary (additions to core)
# -----------------------------------------------

:PropertyDescription a owl:Class ;
    rdfs:subClassOf rdfs:Resource ;
    rdfs:label "Property Description"@en ;
    rdfs:comment "More detailed description of the property, e.g. for specifing sublenses or merging properties."@en ;
    # @@@ work on - rdf:List or :PropertyList...
    rdfs:subClassOf [
        a owl:Restriction ;
        owl:onProperty :alternateProperties ;
        owl:minCardinality "0"^^dtype:nonNegativeInteger ;
    ] ;
    rdfs:subClassOf [
        a owl:Restriction ;
        owl:onProperty :alternateProperties ;
        owl:maxCardinality "1"^^dtype:nonNegativeInteger ;
    ] ;
    rdfs:subClassOf [
        a owl:Restriction ;
        owl:onProperty :alternateProperties ;
        owl:allValuesFrom rdf:List ;
    ] ;
    rdfs:subClassOf [
        a owl:Restriction ;
        owl:onProperty :mergeProperties ;
        owl:minCardinality "0"^^dtype:nonNegativeInteger ;
    ] ;
    rdfs:subClassOf [
        a owl:Restriction ;
        owl:onProperty :mergeProperties ;
        owl:maxCardinality "1"^^dtype:nonNegativeInteger ;
    ] ;
    rdfs:subClassOf [
        a owl:Restriction ;
        owl:onProperty :mergeProperties ;
        owl:allValuesFrom rdf:List ;
    ] ;
    .

# -----------------------------------------------
# Alternate and Merged Properties
# ----------------------------------------------- 

# @@@ is the range an rdf:List or a :PropertyList?
:alternateProperties a owl:ObjectProperty ;
    rdfs:label "alternate properties"@en ;
    rdfs:comment "Defines a sequence of alterntive properties that are used if a property is missing."@en ;
    rdfs:domain :PropertyDescription ;
    rdfs:range rdf:List
    .

:mergeProperties a owl:ObjectProperty ;
    rdfs:label "merge properties"@en ;
    rdfs:comment "The values of all properties in the fresnel:mergeProperties are displayed as one set of property values."@en ; 
    rdfs:domain :PropertyDescription ;
    rdfs:range rdf:List 
    .

# -----------------------------------------------    		
# 3. Lens Relation Vocabulary
# -----------------------------------------------

# @@@ shouldn't this be a purpose?
:moreDetailsFor	a owl:ObjectProperty ;
    rdfs:label "more details for"@en ;
    rdfs:comment "The lens provides more details about an instance than the nother lens.  Good for drill-down."@en ;
    rdfs:domain :Lens ;
    rdfs:range :Lens
    .


# --------------------------------------------------------------   
# Extended Style Vocabulary 
# --------------------------------------------------------------  
# Contents:
#     1. Class and Instance Styles
#     2. Additional Style Description Properties
#     3. Additional Property Value Styles for Media Types
#     4. Style Purposes


# -------------------------------------------------------------- 
# 1. Class and Instance Styles
# --------------------------------------------------------------

# @@@ more work - redefine?
:Format rdfs:subClassOf [
        a owl:Restriction ;
        owl:onProperty :displayAs ;
        owl:minCardinality "0"^^dtype:nonNegativeInteger
    ] ;
    rdfs:subClassOf [
        a owl:Restriction ;
        owl:onProperty :containerStyle ;
        owl:minCardinality "0"^^dtype:nonNegativeInteger
    ]
    .

:displayAs a rdf:Property ;
    rdfs:label "displayAs"@en ;
    rdfs:comment "Specifies how the class is displayed (e.g. image, video)."@en ;
    rdfs:domain :Format ;
    # rdfs:range :LabellingStyle or Literal 
    .
    
:containerStyle a rdf:Property ;
    rdfs:label "container style"@en ;
    rdfs:comment ""@en ;
    rdfs:domain :Format ;
    .

# -------------------------------------------------------------- 
# 2. Additional Style Description Properties
# -------------------------------------------------------------- 

# @@@ more?  redefine?
:StyleDescription rdfs:subClassOf [
        a owl:Restriction ; 
        owl:onProperty :contentReplace ;
        owl:minCardinality "0"^^dtype:nonNegativeInteger ;
    ] ;
    rdfs:subClassOf [
        a owl:Restriction ; 
        owl:onProperty :contentReplace ;
        owl:maxCardinality "1"^^dtype:nonNegativeInteger
    ]
    .

:contentReplace a owl:DatatypeProperty ;
    rdfs:label "content replace"@en ;
    rdfs:comment "Replaces the content of the current box with the specified content."@en  ;
    rdfs:domain :StyleDescription ;
    rdfs:range dtype:string
    .

# @@@ these are datatype properties?
:link a owl:DatatypeProperty ;
    rdfs:label "link"@en ;
    rdfs:comment "The :link pseudo-class applies to all links."@en  ;
    rdfs:domain :StyleDescription ;
    rdfs:range dtype:string
    .

:visited a owl:DatatypeProperty ;
    rdfs:label "visited"@en ;
    rdfs:comment "The :visited pseudo-class applies to all visited links."@en  ;
    rdfs:domain :StyleDescription ;
    rdfs:range dtype:string
    . 

:firstLetter a owl:DatatypeProperty ;
    rdfs:label "first letter"@en ;
    rdfs:comment "The :firstLetter pseudo-class allows you to style the first letter of a text."@en  ;
    rdfs:domain :StyleDescription ;
    rdfs:range dtype:string
    .

:active a owl:DatatypeProperty ;
    rdfs:label "active"@en ;
    rdfs:comment "The active pseudo-class applies while an element is being activated by the user. For example, between the times the user presses the mouse button and releases it."@en  ;
    rdfs:domain :StyleDescription ;
    rdfs:range dtype:string
    . 

:hover a owl:DatatypeProperty ;
    rdfs:label "hover"@en ;
    rdfs:comment "The :hover pseudo-class applies while the user designates an element (with some pointing device), but does not activate it."@en  ;
    rdfs:domain :StyleDescription ;
    rdfs:range dtype:string
    .

:focus a owl:DatatypeProperty ;
    rdfs:label "focus"@en ;
    rdfs:comment "The :focus pseudo-class applies while an element has the focus (accepts keyboard or mouse events, or other forms of input)."@en  ;
    rdfs:domain :StyleDescription ;
    rdfs:range dtype:string
    .

# @@@ needs work
:labelOfParent a owl:Thing ;
    rdfs:label "label of parent"@en ;
    rdfs:comment "Displayes the label of the partent resource, if lenses are related using the sublens property.  fresnel:labelOfParent can be used as property value for fresnel:contentBefore, fresnel:contentAfter, fresnel:contentFirst, fresnel:contentLast.  This might be useful when rendering large graphs."@en
    .

# --------------------------------------------------------------   
# 3. Additional Property Value Styles for Media Types
# --------------------------------------------------------------  

:video a :PropertyValueStyle ;
    rdfs:label "video"@en ;
    rdfs:comment "Retrieve the resource named by the property value and play it as an video clip."@en
    .			

:audio a :PropertyValueStyle ;
    rdfs:label "audio"@en ;
    rdfs:comment "Retrieve the resource named by the property value and play it as an audio clip."@en
    .	

:animation a :PropertyValueStyle ;
    rdfs:label "animation"@en ;
    rdfs:comment "Retrieve the resource named by the property value and display it as animated vector graphics or other animated format."@en
    .			

:text a :PropertyValueStyle ;
    rdfs:label "animation"@en ;
    rdfs:comment "Retrieve the resource named by the property value and display it as text format, such as PDF or MS word using an appropriate viewer."@en
    .

:textstream a :PropertyValueStyle ;
    rdfs:label "animation"@en ;
    rdfs:comment "Retrieve the resource named by the property value and display it as textstream using an appropriate viewer."@en
    .			

:html a :PropertyValueStyle ;
    rdfs:label "animation"@en ;
    rdfs:comment "Retrieve an HTML document and display its body element inside the rendered output document."@en
    .

# -------------------------------------------------------------- 
# 4. Style Purposes
# --------------------------------------------------------------

:screen 	a :Purpose ;
    rdfs:label "screen"@en ;
    rdfs:comment "Intended primarily for color computer screens."@en 
    .

:projection a :Purpose ;
    rdfs:label "Label Lens"@en ;
    rdfs:comment "Intended for projected presentations, for example projectors or print to transparencies."@en 
    .

:print a :Purpose ;
    rdfs:label "Label Lens"@en ;
    rdfs:comment "Intended for paged, opaque material and for documents viewed on screen in print preview mode."@en 
    .					


:stylesheetLink a owl:ObjectProperty ;
    rdfs:label "sylesheet link"@en ;
    rdfs:comment "Reference to an external CSS stylesheet that works with the CSS classes or other instructions used in the group."@en ;
    rdfs:domain :Group ;
    rdfs:range rdfs:Resource
    .

# -----------------------------------------------
# Datatypes
# -----------------------------------------------  
:fslSelector a rdfs:Datatype ;
    rdfs:subClassOf rdfs:Literal ;
    rdfs:isDefinedBy <http://www.w3.org/2004/09/fresnel> ;
    rdfs:label "fslSelector" ;
    rdfs:comment "Fresnel Selector Language (FSL) Selector datatype"@en .

:sparqlSelector a rdfs:Datatype ;
    rdfs:subClassOf rdfs:Literal ;
    rdfs:isDefinedBy <http://www.w3.org/2004/09/fresnel> ;
    rdfs:label "sparqlSelector" ;
    rdfs:comment "SPARQL Selector datatype"@en .

:stylingInstructions a rdfs:Datatype ;
    rdfs:subClassOf rdfs:Literal ;
    rdfs:isDefinedBy <http://www.w3.org/2004/09/fresnel> ;
    rdfs:label "stylingInstructions" ;
    rdfs:comment "Styling instructions (i.e., CSS styling instructions)"@en .    

:styleClass a rdfs:Datatype ;
    rdfs:subClassOf rdfs:Literal ;
    rdfs:isDefinedBy <http://www.w3.org/2004/09/fresnel> ;
    rdfs:label "styleClass" ;
    rdfs:comment "Style class (i.e., HTML class names)"@en .
