@prefix rdf:        <http://www.w3.org/1999/02/22-rdf-syntax-ns#> .
@prefix rdfs:       <http://www.w3.org/2000/01/rdf-schema#> .
@prefix dc:         <http://purl.org/dc/elements/1.1/> .
@prefix dtype:      <http://www.w3.org/2001/XMLSchema#> . 

# Lens Namespace
@prefix :           <http://www.w3.org/2004/09/fresnel#> .

## ------------------------------- ##
## Please see core.owl.n3 instead. ##
## ------------------------------- ##

# -----------------------------------------------
# About this document
<> rdfs:comment     "Core Lens Vocabulary"@en^^dtype:string ;
   dc:description   "Vocabulary for defining lenses on RDF resources."@en^^dtype:string ;
   dc:date          "2005-03-24"^^dtype:date ;
   dc:format        "RDF"@en^^dtype:string ;
   dc:author        "Chris Bizer <chris@bizer.de>" ;
   dc:author        "Ryan Lee <ryanlee@w3.org>" ;
   dc:author        "Stefano Mazzocchi <stefanom@mit.edu>" ;
   dc:author        "Emmanuel Pietriga <emmanuel.pietriga@inria.fr>" ;
   dc:identifier    <http://www.w3.org/2004/09/fresnel/lens-core#>
   .   

# --------------------------------------------------------------   
# Core Lens Vocabulary
# --------------------------------------------------------------  
#
# The lens vocabulary is used for defining 
#    - which properties of an RDF resources are displayed.
#    - how they are ordered. 
#
# There are two variations of the vocabulary:
#    - Simple core, which only supports the selection of nodes by name.
#    - Extended core, which also supports the selection of nodes using FresnelSelectors or SPARQL. 
#
# Contents:
#     1. Lens Vocabulary
#     2. Purpose Vocabulary


# -----------------------------------------------
# 1. Lens Vocabulary 
# -----------------------------------------------

:Lens		rdf:type rdfs:Class ;
			rdfs:label "Lens"@en^^dtype:string ;
    		rdfs:comment "Lens for viewing RDF data."@en^^dtype:string 
    		.		
    		
:lensDomain	rdf:type rdf:Property ;
			rdfs:label "Lens Domain"@en^^dtype:string ;
    		rdfs:comment "Specifies that the lens is usable for this class and its subclasses."@en^^dtype:string ;
			rdfs:domain :Lens
			# rdfs:range rdfs:Class or FSL or SPARQL.
			.

:instanceLensDomain	rdf:type rdf:Property ;
			rdfs:label "Instance Lens Domain"@en^^dtype:string ;
    		rdfs:comment "The lens is usable for the specified set of instances."@en^^dtype:string ;
			rdfs:domain :Lens
			# rdfs:range rdfs:Resource or FSL or SPARQL.
			.			
			
:showProperties	rdf:type rdf:Property ;
			rdfs:label "show properties"@en^^dtype:string ;
      		rdfs:comment "Sequence of all properties which should be shown."@en^^dtype:string ;
			rdfs:domain :Lens 
			# rdfs:range rdf:Property, rdf:List
            .

:hideProperties	rdf:type rdf:Property ;
			rdfs:label "hide properties"@en^^dtype:string ;
      		rdfs:comment "Sequence of all properties which should be hidden.  Has to be used together with fresnel:showProperties fresnel:allProperties"@en^^dtype:string ;
			rdfs:domain :Lens 
			# rdfs:range rdf:Property, rdf:List, FresnelSelector or SPARQL
			.		
  
:allProperties rdf:type rdf:Resource ;
			rdfs:label "All Properties"@en^^dtype:string ;
			rdfs:comment "Set of all properties of the current instance, which have not be explicitly named before. "@en^^dtype:string
			.            
            
# -----------------------------------------------
# 2. Purpose Vocabulary					
# -----------------------------------------------

:purpose	rdf:type rdf:Property ;
			rdfs:label "purpose"@en^^dtype:string ;
    		rdfs:comment "Specifies a purpose for which a lens or style might be appropriate."@en^^dtype:string ;
			# rdfs:domain :Lens :Style or :StyleGroup ;
			rdfs:range :Purpose 
            .
            
:Purpose	rdf:type rdfs:Class ;
			rdfs:label "Purpose"@en^^dtype:string ;
    		rdfs:comment "Propose in which a specific lens might be appropriate."@en^^dtype:string
    		.

:defaultLens rdf:type :Purpose ;
			rdfs:label "Default Lens"@en^^dtype:string ;
			rdfs:comment "Provides the browser with a starting point which lens to show."@en^^dtype:string 
			.

:labelLens	rdf:type :Purpose ;
			rdfs:label "Label Lens"@en^^dtype:string ;
			rdfs:comment "Lens for providing a label for a resource."@en^^dtype:string 
			.